proof/correctness/avx2/extraction/jkem_avx2.ec
@@ -947,7 +947,26 @@ W16.of_int 996; W16.of_int 991; W16.of_int 958; W16.of_int 1869;
 W16.of_int 1522; W16.of_int 1628].
 
 
-module M = {
+module type Syscall_t = {
+  proc randombytes_32(_:W8.t Array32.t) : W8.t Array32.t
+  proc randombytes_64(_:W8.t Array64.t) : W8.t Array64.t
+}.
+
+module Syscall : Syscall_t = {
+  proc randombytes_32(a:W8.t Array32.t) : W8.t Array32.t = {
+    a <$ dmap WArray32.darray
+         (fun a => Array32.init (fun i => WArray32.get8 a i));
+    return a;
+  }
+  
+  proc randombytes_64(a:W8.t Array64.t) : W8.t Array64.t = {
+    a <$ dmap WArray64.darray
+         (fun a => Array64.init (fun i => WArray64.get8 a i));
+    return a;
+  }
+}.
+
+module M(SC:Syscall_t) = {
   proc __shuffle8 (a:W256.t, b:W256.t) : W256.t * W256.t = {
     
     var r0:W256.t;
@@ -6527,11 +6546,57 @@ module M = {
                 _shake256_64 (shkp, t64, kr);
                 return ();
               }
+              proc __randombytes64 (randomnessp:W64.t) : unit = {
+                var aux: int;
+                
+                var r:W8.t Array64.t;
+                var rp:W8.t Array64.t;
+                var i:int;
+                var t64:W64.t;
+                r <- witness;
+                rp <- witness;
+                rp <- r;
+                rp <@ SC.randombytes_64 (rp);
+                aux <- (64 %/ 8);
+                i <- 0;
+                while (i < aux) {
+                  t64 <- (get64 (WArray64.init8 (fun i_0 => rp.[i_0])) i);
+                  Glob.mem <-
+                  storeW64 Glob.mem (W64.to_uint (randomnessp + (W64.of_int (8 * i)))) (t64);
+                  i <- i + 1;
+                }
+                return ();
+              }
+              proc __randombytes32 (randomnessp:W64.t) : unit = {
+                var aux: int;
+                
+                var r:W8.t Array32.t;
+                var rp:W8.t Array32.t;
+                var i:int;
+                var t64:W64.t;
+                r <- witness;
+                rp <- witness;
+                rp <- r;
+                rp <@ SC.randombytes_32 (rp);
+                aux <- (32 %/ 8);
+                i <- 0;
+                while (i < aux) {
+                  t64 <- (get64 (WArray32.init8 (fun i_0 => rp.[i_0])) i);
+                  Glob.mem <-
+                  storeW64 Glob.mem (W64.to_uint (randomnessp + (W64.of_int (8 * i)))) (t64);
+                  i <- i + 1;
+                }
+                return ();
+              }
               proc crypto_kem_keypair_jazz (pkp:W64.t, skp:W64.t,
                                             randomnessp:W64.t) : unit = {
                 
                 
                 
+                pkp <- pkp;
+                skp <- skp;
+                randomnessp <- randomnessp;
+                __randombytes64 (randomnessp);
                 __crypto_kem_keypair_jazz (pkp, skp, randomnessp);
                 return ();
               }
@@ -6540,6 +6605,11 @@ module M = {
                 
                 
                 
+                ctp <- ctp;
+                shkp <- shkp;
+                pkp <- pkp;
+                randomnessp <- randomnessp;
+                __randombytes32 (randomnessp);
                 __crypto_kem_enc_jazz (ctp, shkp, pkp, randomnessp);
                 return ();
               }
