proof/correctness/avx2/Kyber_AVX_ref_lowlevel_equivs.ec
@@ -38,7 +38,7 @@ import KyberPolyAVXVec.
 import KyberPolyVecAVXVec.
 
 lemma polyvec_decompress_equiv mem _p :
-    equiv [ M.__polyvec_decompress ~   Jkem.M.__polyvec_decompress  :
+    equiv [Jkem_avx2.M(Jkem_avx2.Syscall).__polyvec_decompress ~  Jkem.M(Jkem.Syscall).__polyvec_decompress  :
              valid_ptr _p (3*320) /\
              Glob.mem{1} = mem /\ to_uint rp{1} = _p /\
              ={Glob.mem} /\ rp{1} = ap{2}
@@ -132,7 +132,7 @@ qed.
 
 
 equiv compressequivvec mem _p : 
-  M.__polyvec_compress ~   Jkem.M.__polyvec_compress :
+ Jkem_avx2.M(Jkem_avx2.Syscall).__polyvec_compress ~  Jkem.M(Jkem.Syscall).__polyvec_compress :
      pos_bound768_cxq a{1} 0 768 2 /\
      pos_bound768_cxq a{2} 0 768 2 /\
     lift_array768 a{1} = lift_array768 a{2} /\ 
@@ -241,7 +241,7 @@ proof.
 qed.
 
 equiv compressequivvec_1 mem : 
-  M.__polyvec_compress_1 ~   Jkem.M.__i_polyvec_compress :
+ Jkem_avx2.M(Jkem_avx2.Syscall).__polyvec_compress_1 ~  Jkem.M(Jkem.Syscall).__i_polyvec_compress :
      pos_bound768_cxq a{1} 0 768 2 /\
      pos_bound768_cxq a{2} 0 768 2 /\
     lift_array768 a{1} = lift_array768 a{2} /\ 
@@ -323,7 +323,7 @@ proof.
 qed.
 
 lemma poly_decompress_equiv mem _p : 
-    equiv [ M._poly_decompress ~   Jkem.M._poly_decompress  :
+    equiv [Jkem_avx2.M(Jkem_avx2.Syscall)._poly_decompress ~  Jkem.M(Jkem.Syscall)._poly_decompress  :
              valid_ptr _p 128 /\
              Glob.mem{1} = mem /\ to_uint ap{1} = _p /\
              ={Glob.mem,ap}
@@ -398,7 +398,7 @@ proof.
 qed.
 
 equiv compressequiv_1 mem : 
-  M._poly_compress_1 ~   Jkem.M._i_poly_compress :
+ Jkem_avx2.M(Jkem_avx2.Syscall)._poly_compress_1 ~  Jkem.M(Jkem.Syscall)._i_poly_compress :
      pos_bound256_cxq a{1} 0 256 2 /\
      pos_bound256_cxq a{2} 0 256 2 /\
     lift_array256 a{1} = lift_array256 a{2} /\ 
@@ -469,7 +469,7 @@ proof.
 qed.
 
 equiv compressequiv mem _p : 
-  M._poly_compress ~   Jkem.M._poly_compress :
+ Jkem_avx2.M(Jkem_avx2.Syscall)._poly_compress ~  Jkem.M(Jkem.Syscall)._poly_compress :
      pos_bound256_cxq a{1} 0 256 2 /\
      pos_bound256_cxq a{2} 0 256 2 /\
     lift_array256 a{1} = lift_array256 a{2} /\ 
@@ -567,7 +567,7 @@ qed.
 lemma subequiv_noperm  (ab bb : int):
     0 <= ab && ab <= 6 =>
     0 <= bb && bb <= 3 =>
-    equiv [ M._poly_sub ~ Jkem.M._poly_sub :
+    equiv [Jkem_avx2.M(Jkem_avx2.Syscall)._poly_sub ~Jkem.M(Jkem.Syscall)._poly_sub :
       lift_array256 ap{1} = lift_array256 ( ap{2}) /\
       lift_array256 bp{1} = lift_array256 ( bp{2}) /\
       signed_bound_cxq ap{2} 0 256 ab /\ 
@@ -654,7 +654,7 @@ move : HHH; move : (W16.to_uint_cmp x); move :  (W16.to_uint_cmp y) => /=; smt()
 qed.
 
 equiv frommontequiv : 
-  M._poly_frommont ~   Jkem.M._poly_frommont :
+ Jkem_avx2.M(Jkem_avx2.Syscall)._poly_frommont ~  Jkem.M(Jkem.Syscall)._poly_frommont :
     lift_array256 arg{1} = nttunpack (lift_array256 arg{2}) ==> 
     lift_array256 res{1} = nttunpack (lift_array256 res{2}) /\
     signed_bound_cxq res{1} 0 256 2 /\ 
@@ -723,7 +723,7 @@ do split.
 qed.
 
 equiv reduceequiv : 
-  M.__poly_reduce ~   Jkem.M.__poly_reduce :
+ Jkem_avx2.M(Jkem_avx2.Syscall).__poly_reduce ~  Jkem.M(Jkem.Syscall).__poly_reduce :
     lift_array256 arg{1} = nttunpack (lift_array256 arg{2}) ==> 
     lift_array256 res{1} = nttunpack (lift_array256 res{2}) /\
     pos_bound256_cxq res{1} 0 256 2 /\ 
@@ -753,7 +753,7 @@ smt(Array256.mapiE nttunpack_bnd Array256.allP).
 qed.
 
 equiv reduceequiv_noperm : 
-  M.__poly_reduce ~   Jkem.M.__poly_reduce :
+ Jkem_avx2.M(Jkem_avx2.Syscall).__poly_reduce ~  Jkem.M(Jkem.Syscall).__poly_reduce :
     lift_array256 arg{1} = lift_array256 arg{2} ==> 
     lift_array256 res{1} = lift_array256 res{2} /\
     pos_bound256_cxq res{1} 0 256 2 /\ 
@@ -786,7 +786,7 @@ import Zq.
 require import NTT_AVX_j.
 
 equiv basemulequiv : 
-  M._poly_basemul ~ Jkem.M._poly_basemul :
+ Jkem_avx2.M(Jkem_avx2.Syscall)._poly_basemul ~Jkem.M(Jkem.Syscall)._poly_basemul :
     lift_array256 ap{1} = nttunpack (lift_array256 ap{2}) /\
     lift_array256 bp{1} = nttunpack (lift_array256 bp{2}) /\
     signed_bound_cxq ap{1} 0 256 2 /\  
@@ -826,7 +826,7 @@ lemma addequiv  (ab1 bb1 ab2 bb2 : int):
     0 <= ab2 && ab2 <= 6 =>
     0 <= bb1 && bb1 <= 3 =>
     0 <= bb2 && bb2 <= 3 =>
-    equiv [ M._poly_add2 ~ Jkem.M._poly_add2 :
+    equiv [Jkem_avx2.M(Jkem_avx2.Syscall)._poly_add2 ~Jkem.M(Jkem.Syscall)._poly_add2 :
       lift_array256 rp{1} = lift_array256 (nttunpack rp{2}) /\
       lift_array256 bp{1} = lift_array256 (nttunpack bp{2}) /\
       signed_bound_cxq rp{2} 0 256 ab2 /\ 
@@ -877,7 +877,7 @@ qed.
 lemma addequiv_noperm  (ab bb : int):
     0 <= ab && ab <= 6 =>
     0 <= bb && bb <= 3 =>
-    equiv [ M._poly_add2 ~ Jkem.M._poly_add2 :
+    equiv [Jkem_avx2.M(Jkem_avx2.Syscall)._poly_add2 ~Jkem.M(Jkem.Syscall)._poly_add2 :
       lift_array256 rp{1} = lift_array256 ( rp{2}) /\
       lift_array256 bp{1} = lift_array256 ( bp{2}) /\
       signed_bound_cxq rp{2} 0 256 ab /\ 
@@ -917,7 +917,7 @@ rewrite H7 // H9 /#.
 qed.
 
 equiv frommsgequiv_noperm  : 
-  M._poly_frommsg_1 ~   Jkem.M._i_poly_frommsg :
+ Jkem_avx2.M(Jkem_avx2.Syscall)._poly_frommsg_1 ~  Jkem.M(Jkem.Syscall)._i_poly_frommsg :
     ={ap} ==> 
     lift_array256 res{1} = lift_array256 res{2} /\
     pos_bound256_cxq res{1} 0 256 1 /\ 
@@ -957,7 +957,7 @@ lemma compress_poly_rng i xs :
 rewrite /compress_poly /map allP => Hi j Hj. rewrite !initiE //=. rewrite compress_rng //. qed.
 
 equiv tomsgequiv_noperm  : 
-  M._poly_tomsg_1 ~   Jkem.M._i_poly_tomsg :
+ Jkem_avx2.M(Jkem_avx2.Syscall)._poly_tomsg_1 ~  Jkem.M(Jkem.Syscall)._i_poly_tomsg :
     lift_array256 a{1} = lift_array256 a{2} /\
     pos_bound256_cxq a{1} 0 256 2 /\ 
     pos_bound256_cxq a{2} 0 256 2 ==>
@@ -997,7 +997,7 @@ qed.
 
 lemma polyvec_tobytes_equiv :
     forall (_p : int),
-    equiv [ Jkem_avx2.M.__polyvec_tobytes ~ Jkem.M.__polyvec_tobytes :
+    equiv [Jkem_avx2.M(Jkem_avx2.Syscall).__polyvec_tobytes ~Jkem.M(Jkem.Syscall).__polyvec_tobytes :
              _p = to_uint rp{1} /\
              valid_ptr (W64.to_uint rp{1}) (3*384) /\
              pos_bound768_cxq a{1} 0 768 2 /\
@@ -1107,7 +1107,7 @@ lemma polyvec_add2_equiv  (ab bb : int):
     0 <= ab && ab <= 6 =>
     0 <= bb && bb <= 3 =>
   forall (_a _b : Fq Array768.t),
-    equiv [ Jkem_avx2.M.__polyvec_add2 ~ Jkem.M.__polyvec_add2 :
+    equiv [Jkem_avx2.M(Jkem_avx2.Syscall).__polyvec_add2 ~Jkem.M(Jkem.Syscall).__polyvec_add2 :
       _a = lift_array768 r{2} /\
       _b = lift_array768 b{2} /\ signed_bound768_cxq r{2} 0 768 ab /\ signed_bound768_cxq b{2} 0 768 bb /\
       _a = nttpackv (lift_array768 r{1}) /\
@@ -1188,7 +1188,7 @@ lemma polyvec_add2_equiv_noperm  (ab bb : int):
     0 <= ab && ab <= 6 =>
     0 <= bb && bb <= 3 =>
   forall (_a _b : Fq Array768.t),
-    equiv [ Jkem_avx2.M.__polyvec_add2 ~ Jkem.M.__polyvec_add2 :
+    equiv [Jkem_avx2.M(Jkem_avx2.Syscall).__polyvec_add2 ~Jkem.M(Jkem.Syscall).__polyvec_add2 :
       _a = lift_array768 r{2} /\
       _b = lift_array768 b{2} /\ signed_bound768_cxq r{2} 0 768 ab /\ signed_bound768_cxq b{2} 0 768 bb /\
       _a = lift_array768 r{1} /\
@@ -1219,7 +1219,7 @@ rewrite !mapiE;smt(Array768.mapiE).
 qed.
 
 lemma polyvec_reduce_equiv _a :
-    equiv [ Jkem_avx2.M.__polyvec_reduce ~ Jkem.M.__polyvec_reduce :
+    equiv [Jkem_avx2.M(Jkem_avx2.Syscall).__polyvec_reduce ~Jkem.M(Jkem.Syscall).__polyvec_reduce :
        _a  = lift_array768 r{2} /\  _a  = nttpackv (lift_array768 r{1})  ==>
        (forall k, 0 <= k < 768 => bpos16 res{1}.[k] (2*q)) /\
        (forall k, 0 <= k < 768 => bpos16 res{2}.[k] (2*q)) /\
@@ -1242,7 +1242,7 @@ smt(packvK unpackvK).
 qed.
 
 lemma polyvec_reduce_equiv_noperm _a :
-    equiv [ Jkem_avx2.M.__polyvec_reduce ~ Jkem.M.__polyvec_reduce :
+    equiv [Jkem_avx2.M(Jkem_avx2.Syscall).__polyvec_reduce ~Jkem.M(Jkem.Syscall).__polyvec_reduce :
        _a  = lift_array768 r{2} /\  _a  = lift_array768 r{1}  ==>
        (forall k, 0 <= k < 768 => bpos16 res{1}.[k] (2*q)) /\
        (forall k, 0 <= k < 768 => bpos16 res{2}.[k] (2*q)) /\
@@ -1262,7 +1262,7 @@ auto => /> /#.
 qed.
 
 equiv pointwiseequiv : 
-  M.__polyvec_pointwise_acc ~   Jkem.M.__polyvec_pointwise_acc :
+ Jkem_avx2.M(Jkem_avx2.Syscall).__polyvec_pointwise_acc ~  Jkem.M(Jkem.Syscall).__polyvec_pointwise_acc :
     lift_array768 arg{1}.`2 = nttunpackv (lift_array768 arg{2}.`1) /\
     lift_array768 arg{1}.`3 = nttunpackv (lift_array768 arg{2}.`2) /\
     signed_bound768_cxq arg{1}.`2 0 768 2 /\
@@ -1393,7 +1393,7 @@ smt().
 qed.
 
 equiv nttequiv :
- Jkem_avx2.M.__polyvec_ntt ~ Jkem.M.__polyvec_ntt : 
+Jkem_avx2.M(Jkem_avx2.Syscall).__polyvec_ntt ~Jkem.M(Jkem.Syscall).__polyvec_ntt : 
    lift_array768 arg{1} = lift_array768 arg{2} /\ 
    signed_bound768_cxq arg{1} 0 768 2 /\ 
    signed_bound768_cxq arg{2} 0 768 2 ==>
@@ -1462,7 +1462,7 @@ move : (Hidx (k-512) _)=>//; smt(mem_iota).
 qed.
 
 equiv polyinvnttequiv :
- Jkem_avx2.M._poly_invntt ~ Jkem.M._poly_invntt : 
+Jkem_avx2.M(Jkem_avx2.Syscall)._poly_invntt ~Jkem.M(Jkem.Syscall)._poly_invntt : 
    lift_array256 arg{1} = nttunpack (lift_array256 arg{2}) /\ 
    signed_bound_cxq arg{1} 0 256 4 /\ 
    signed_bound_cxq arg{2} 0 256 4 ==>
@@ -1486,7 +1486,7 @@ lemma eq_vectorP3 :
 smt(KMatrix.Vector.eq_vectorP). qed.
 
 equiv invnttequiv :
- Jkem_avx2.M.__polyvec_invntt ~ Jkem.M.__polyvec_invntt : 
+Jkem_avx2.M(Jkem_avx2.Syscall).__polyvec_invntt ~Jkem.M(Jkem.Syscall).__polyvec_invntt : 
    lift_array768 arg{1} = nttunpackv (lift_array768 arg{2}) /\ 
    signed_bound768_cxq arg{1} 0 768 4 /\ 
    signed_bound768_cxq arg{2} 0 768 4 ==>
